sliding set model

newLibrary/sbf-model.dfy
@@ -22,6 +22,50 @@
                     (t < t' <= t + paneCycleTime)  ==> (query(k) @ t == true)
 */
 
+
+/*
+    What do we want to prove?
+    Is it along the lines of:
+        lastInsertTime[key] >= (curTs - tInterval) 
+            ==> (exists(active, key) || exists(maintain, key))
+
+    How do we even specify this...
+
+*/
+
+/*
+TODO: 
+
+we need to straighten out the time / timestamp / rollover logic.
+
+*/
+
+          /*
+                assume curTs + delay == tlastRotate
+                0 < delay < max32 (so no rollover)
+                
+                curTs == tlastRotate - delay
+
+                that's impossible. time can't move backwards...
+
+
+
+
+                curTs - tLastRotate 
+
+                This is really complicated, just as complicated as reasoning about timing 
+                in the full case study. 
+
+                So we have to find a way to simplify. 
+
+                    Is there an easier way to determine when to switch panes, besides looking at the "time"?
+                    And how DO they do it? in verifiable p4?
+
+                    Or will self clocking work?
+
+            */
+
+
 include "verifiableLucid.dfy"
 
 module SlidingBloomFilter refines VerifiableLucid {
@@ -30,12 +74,15 @@ module SlidingBloomFilter refines VerifiableLucid {
         const seed0 : uint32 := 7
         const seed1 : uint32 := 13
 
+        var curTs : uint32
+
         // interval between switching panes
         // we need to see at least nRows packets during this 
         // interval, to clear each entry in the expired pane.
         // lets say its 10 * nRows, which means that 
         // we must see 1 packet every 10 time units.
-        const tinterval : uint32 := 10 * nRows
+        const tPktInterArrival : uint32 := 10
+        const tinterval : uint32 := tPktInterArrival * nRows
 
         var tLastRotate : uint32 // time of last rotation
         var activePane : uint32 // which pane is active
@@ -48,7 +95,26 @@ module SlidingBloomFilter refines VerifiableLucid {
         var p1col1 : seq<uint32>  // maintaining pane, column 1
         var p2col0 : seq<uint32>  // clearing pane, column 0
         var p2col1 : seq<uint32>  // clearing pane, column 1
-        
+
+        ghost var lastInsertTime : map<uint32, nat> // last key insertion
+        ghost var lastOpTime : nat // last operation execution time
+
+        predicate arraySizes ()
+        reads this`p0col0, this`p0col1, this`p1col0, this`p1col1, this`p2col0, this`p2col1
+        {
+               |p0col0| == nRows && |p0col1| == nRows
+            && |p1col0| == nRows && |p1col1| == nRows
+            && |p2col0| == nRows && |p2col1| == nRows
+        }
+
+        twostate predicate arraySizesUnchanged ()
+        reads this`p0col0, this`p0col1, this`p1col0, this`p1col1, this`p2col0, this`p2col1
+        {
+               |p0col0| == |old(p0col0)| && |p0col1| == |old(p0col1)|
+            && |p1col0| == |old(p1col0)| && |p1col1| == |old(p1col1)|
+            && |p2col0| == |old(p2col0)| && |p2col1| == |old(p2col1)|
+        }
+
         constructor ()
             ensures tLastRotate == 0
             ensures activePane == 0
@@ -57,6 +123,9 @@ module SlidingBloomFilter refines VerifiableLucid {
             ensures p1col0 == zeros(nRows) && p1col1 == zeros(nRows)
             ensures p2col0 == zeros(nRows) && p2col1 == zeros(nRows)
             ensures fresh(this)
+            ensures lastInsertTime == map[]
+            ensures lastOpTime == 0
+            ensures curTs == 0
         {
             tLastRotate := 0;
             activePane := 0;
@@ -67,6 +136,9 @@ module SlidingBloomFilter refines VerifiableLucid {
             p1col1 := zeros(nRows);
             p2col0 := zeros(nRows);
             p2col1 := zeros(nRows);
+            lastInsertTime := map[];
+            lastOpTime := 0;
+            curTs := 0;
         }
 
         function hash(seed : uint32, key : uint32) : uint32
@@ -78,15 +150,15 @@ module SlidingBloomFilter refines VerifiableLucid {
         // memory operations that we want to be atomic in final version
 
         // update the time since rotate. 
-        // if time since tLastRotate is greater than tinterval, return curTime
-        function updateIfTimeElapsed(lastTime : uint32, curTime : uint32) : uint32
-        {
-            if (curTime - lastTime >= tinterval) then (
-                curTime
-             ) else (
-                lastTime
-            )
-        }
+        // if time since tLastRotate is greater than tinterval, return curTs
+        // function updateIfTimeElapsed(lastTime : uint32, t : uint32) : uint32
+        // {
+        //     if (t - lastTime >= tinterval) then (
+        //         t
+        //      ) else (
+        //         lastTime
+        //     )
+        // }
         // update the active pane.
         function updateActivePane(storedVal : uint32, unused : uint32) : uint32
             requires 0 <= storedVal < 3
@@ -102,6 +174,68 @@ module SlidingBloomFilter refines VerifiableLucid {
             if (storedVal == nRows - 1) then 0 else (storedVal + 1)
         }
 
+        function nextActive(curActive : uint32) : uint32
+            requires 0 <= curActive < 3
+        {
+            match curActive {
+                case 2 => 0
+                case _ => curActive + 1
+            }
+        }
+
+        twostate predicate rotatesOnlyAfterInterval()
+            reads this`curTs, this`activePane, this`tLastRotate
+        {
+            (0 <= old(activePane) < 3) &&
+            if   ((curTs - old(tLastRotate)) % max32 >= tinterval)
+            then (activePane == nextActive(old(activePane)) && (tLastRotate == curTs % max32))
+            else (activePane == old(activePane) && tLastRotate == old(tLastRotate))
+        }
+
+        ghost predicate timingInvariant()
+            reads this`curTs, this`lastOpTime
+        { 
+            ((curTs - lastOpTime) % max32) <= tPktInterArrival 
+        }
+
+        predicate stateInvariant()
+            reads this`activePane, this`clearIdx
+        {
+            0 <= activePane < 3
+            && 0 <= clearIdx < nRows
+        }
+
+        predicate clearingPaneAtIndexIsZero()
+            reads this`activePane, this`clearIdx
+            reads this`p0col0, this`p0col1, this`p1col0, this`p1col1, this`p2col0, this`p2col1
+            requires arraySizes ()
+            requires 0 <= clearIdx < nRows
+            requires 0 <= activePane < 3
+        {
+            match activePane {
+                case 0 => p1col0[clearIdx] == 0 && p1col1[clearIdx] == 0
+                case 1 => p2col0[clearIdx] == 0 && p2col1[clearIdx] == 0
+                case 2 => p0col0[clearIdx] == 0 && p0col0[clearIdx] == 0
+            }
+        }
+
+        predicate foundIfSetInActiveOrMaintained(key : uint32)
+            reads this`activePane
+            reads this`p0col0, this`p0col1, this`p1col0, this`p1col1, this`p2col0, this`p2col1
+            requires arraySizes ()
+            requires 0 <= activePane < 3
+        {
+            match activePane {
+                case 0 => 
+                    keyExistsInPane(key, 0) || keyExistsInPane(key, 2)
+                case 1 =>
+                    keyExistsInPane(key, 1) || keyExistsInPane(key, 0)
+                case 2 =>
+                    keyExistsInPane(key, 2) || keyExistsInPane(key, 1)
+            }
+        }
+
+
         /* 
             query reads from the active pane and the maintaining pane,
             and writes to the clearing pane.
@@ -110,27 +244,52 @@ module SlidingBloomFilter refines VerifiableLucid {
         */
         method query(key : uint32)
             returns (res : uint32)
-            requires 0 <= activePane < 3
-            requires 0 <= clearIdx < nRows
-            requires |p0col0| == nRows && |p0col1| == nRows
-            requires |p1col0| == nRows && |p1col1| == nRows
-            requires |p2col0| == nRows && |p2col1| == nRows
+            requires tLastRotate != curTs // I think this is always true.
+            requires timingInvariant ()
+            requires stateInvariant ()
+            requires arraySizes ()
             modifies this`activePane, this`clearIdx, this`tLastRotate
             modifies this`p0col0, this`p0col1, this`p1col0, this`p1col1, this`p2col0, this`p2col1
-            ensures 0 <= activePane < 3
-            ensures 0 <= clearIdx < nRows
+            modifies this`lastOpTime
+            ensures lastOpTime == curTs
+            ensures stateInvariant ()
+            ensures arraySizesUnchanged ()
+            ensures rotatesOnlyAfterInterval () // rotation correctness
+            ensures noRemovalsInActiveOrMaintain () // maintenence correctness
+            ensures clearingPaneAtIndexIsZero () // clearing correctness -- not complete.. but maybe sufficient?
+            ensures foundIfSetInActiveOrMaintained(key) <==> res == 1
         {
-            // 1. calculate time since last rotation. 
-            //    if it's greater than tinterval, 
-            //    rotate panes and update tLastRotate
-            tLastRotate := updateIfTimeElapsed(tLastRotate, curTimestamp);
-            // we are rotating now
-            if (tLastRotate == curTimestamp) {
+            // Question: is it possible for tLastRotate to be 
+            // the current timestamp, when the method begins?
+            // Answer: No. Because tinterval << max32, and we know we get at least 
+            // one message every tinterval.
+            // that would require us to not have gotten 
+            // any messages since the last rotation interval
+            // Bigger question: is there a simpler way to determine when to rotate?
+            // and / or is tLastRotate the right thing to track?
+
+            /*
+                you could track time since rotate directly?
+                packetInterarrival = timestamp - lasttimestamp;
+                tSinceRotate = tSinceRotate + packetInterarrival;
+                if (tSinceRotate >= tinterval) {
+                    tSinceRotate = 0;
+                }
+            */
+
+            // 1. calculate time since last rotation
+            var t_since_last_rotate : uint32 := (curTs - tLastRotate) % max32;
+            // rotate and update index, or just update index
+            if (t_since_last_rotate >= tinterval) {
+                tLastRotate := curTs;
                 activePane := updateActivePane(activePane, 0);
                 clearIdx := 0;
+                assert rotatesOnlyAfterInterval ();
             } else {
+
                 clearIdx := updateClearIdx(clearIdx, 0);
             }
+
             // 2. read from the active and maintaining panes, clear the clearing pane
             var h0 := hash(seed0, key);
             var h1 := hash(seed1, key);
@@ -138,84 +297,227 @@ module SlidingBloomFilter refines VerifiableLucid {
             var a1 := 0;
             var m0 := 0;
             var m1 := 0;
+            // activePane 0 ==> pane roles = [active, clearing, maintaining]
+            // activePane 1 ==> pane roles = [maintaining, active, clearing]
+            // activePane 2 ==> pane roles = [clearing, maintaining, active]
             if (activePane == 0) {
-                // read active and maintaining
+                // active = 0, maintaining = 2, clearing = 1
                 a0 := p0col0[h0];
                 a1 := p0col1[h1];
-                m0 := p1col0[h0];
-                m1 := p1col1[h1];
-                // clear stale
-                p2col0 := p2col0[clearIdx := 0];
-                p2col1 := p2col1[clearIdx := 0];
-            } else if (activePane == 1) {
-                // read active and maintaining
-                a0 := p1col0[h0];
-                a1 := p1col1[h1];
-                m0 := p2col0[h0];
-                m1 := p2col1[h1];
-                // clear stale
-                p0col0 := p0col0[clearIdx := 0];
-                p0col1 := p0col1[clearIdx := 0];
-            } else {
-                // read active and maintaining
-                a0 := p2col0[h0];
-                a1 := p2col1[h1];
-                m0 := p0col0[h0];
-                m1 := p0col1[h1];
-                // clear stale
                 p1col0 := p1col0[clearIdx := 0];
                 p1col1 := p1col1[clearIdx := 0];
+                m0 := p2col0[h0];
+                m1 := p2col1[h1];
+            } else if (activePane == 1) {
+                // active = 1, maintaining = 0, clearing = 2
+                m0 := p0col0[h0]; 
+                m1 := p0col1[h1];
+                a0 := p1col0[h0];
+                a1 := p1col1[h1];
+                p2col0 := p2col0[clearIdx := 0];
+                p2col1 := p2col1[clearIdx := 0];
+            } else {
+                // active = 2, maintaining = 1, clearing = 0
+                p0col0 := p0col0[clearIdx := 0];
+                p0col1 := p0col1[clearIdx := 0];
+                m0 := p1col0[h0];
+                m1 := p1col1[h1];
+                a0 := p2col0[h0];
+                a1 := p2col1[h1];
             }
             // 3. calculate result: AND columns in same pane, OR across panes
             res := 0;
             if ((a0 == 1 && a1 == 1) || (m0 == 1 && m1 == 1)) {
                 res := 1;
             }
+            lastOpTime := curTs;
+        }
+
+        // A key exists in a pane
+        predicate keyExistsIn(c0 : seq<uint32>, c1 : seq<uint32>, key : uint32)
+            requires |c0| == nRows && |c1| == nRows            
+        {
+            c0[hash(seed0, key)] == 1 && c1[hash(seed1, key)] == 1
+        }
+
+        predicate keyExistsInActive(key : uint32)
+            reads this`p0col0, this`p0col1, this`p1col0, this`p1col1, this`p2col0, this`p2col1
+            reads this`activePane
+            requires 0 <= activePane < 3
+        {
+            arraySizes () &&
+            match activePane {
+                case 0 => keyExistsIn(p0col0, p0col1, key)
+                case 1 => keyExistsIn(p1col0, p1col1, key)
+                case 2 => keyExistsIn(p2col0, p2col1, key)
+            }
+        }
+        predicate keyExistsInPane(key : uint32, pane : uint32)
+            reads this`p0col0, this`p0col1, this`p1col0, this`p1col1, this`p2col0, this`p2col1
+            requires 0 <= pane < 3
+        {
+            arraySizes () &&
+            match pane {
+                case 0 => keyExistsIn(p0col0, p0col1, key)
+                case 1 => keyExistsIn(p1col0, p1col1, key)
+                case 2 => keyExistsIn(p2col0, p2col1, key)
+            }
+        }
+
+
+        predicate onesPreserved(oldCols : seq<uint32>, cols : seq<uint32>)
+        requires |cols| == |oldCols|
+        {
+            forall i :: 0 <= i < |cols| && oldCols[i] == 1 ==> cols[i] == 1
+        }
+
+        twostate predicate noRemovalsInActiveOrMaintain()
+            reads this`p0col0, this`p0col1, this`p1col0, this`p1col1, this`p2col0, this`p2col1
+            reads this`activePane
+            requires 0 <= activePane < 3
+        {
+            arraySizesUnchanged() &&
+            match activePane {
+                case 0 => onesPreserved(old(p0col0), p0col0) && onesPreserved(old(p0col1), p0col1) 
+                       && onesPreserved(old(p2col0), p2col0) && onesPreserved(old(p2col1), p2col1)
+                case 1 => onesPreserved(old(p1col0), p1col0) && onesPreserved(old(p1col1), p1col1) 
+                       && onesPreserved(old(p0col0), p0col0) && onesPreserved(old(p0col1), p0col1)
+                case 2 => onesPreserved(old(p2col0), p2col0) && onesPreserved(old(p2col1), p2col1) 
+                       && onesPreserved(old(p1col0), p1col0) && onesPreserved(old(p1col1), p1col1)
+            }
         }
 
         method insert(key : uint32)
-            requires 0 <= activePane < 3 
-            requires 0 <= clearIdx < nRows
-            requires |p0col0| == nRows && |p0col1| == nRows
-            requires |p1col0| == nRows && |p1col1| == nRows
-            requires |p2col0| == nRows && |p2col1| == nRows
             modifies this`tLastRotate, this`activePane, this`clearIdx
             modifies this`p0col0, this`p0col1, this`p1col0, this`p1col1, this`p2col0, this`p2col1
-            ensures 0 <= activePane < 3
-            ensures 0 <= clearIdx < nRows
+            modifies this`lastInsertTime, this`lastOpTime
+            requires timingInvariant ()
+            requires stateInvariant ()
+            requires arraySizes ()
+            ensures lastOpTime == curTs
+            ensures stateInvariant ()
+            ensures arraySizesUnchanged ()
+            ensures clearingPaneAtIndexIsZero ()
+            ensures rotatesOnlyAfterInterval () // rotation correctness
+            ensures keyExistsInActive(key) // insertion correctness
+            ensures noRemovalsInActiveOrMaintain() // maintenence correctness
+            ensures lastInsertTime == old(lastInsertTime)[key := curTs] // ghost insert time update correctness
         {
-            /* 1. calculate time since last rotation. 
-                    - if it's greater than tinterval, 
-                      rotate panes and update tLastRotate */
-            tLastRotate := updateIfTimeElapsed(tLastRotate, curTimestamp);
-            // we are rotating now
-            if (tLastRotate == curTimestamp) {
+            // 1. calculate time since last rotation
+            var t_since_last_rotate : uint32 := (curTs - tLastRotate) % max32;
+            // rotate and update index, or just update index
+            if (t_since_last_rotate >= tinterval) {
+                tLastRotate := curTs % max32;
                 activePane := updateActivePane(activePane, 0);
                 clearIdx := 0;
             } else {
                 clearIdx := updateClearIdx(clearIdx, 0);
             }
+
             // 2. write to the active pane at hash indices, 
             //    clear the clearing pane at clearIdx
+            // activePane 0 ==> pane roles = [active, clearing, maintaining]
+            // activePane 1 ==> pane roles = [maintaining, active, clearing]
+            // activePane 2 ==> pane roles = [clearing, maintaining, active]
             var h0 := hash(seed0, key);
             var h1 := hash(seed1, key);
             if (activePane == 0) {
                 p0col0 := p0col0[h0 := 1];
                 p0col1 := p0col1[h1 := 1];
-                p2col0 := p2col0[clearIdx := 0];
-                p2col1 := p2col1[clearIdx := 0];
-            } else if (activePane == 1) {
-                p0col0 := p0col0[clearIdx := 0];
-                p0col1 := p0col1[clearIdx := 0];
-                p1col0 := p1col0[h0 := 1];
-                p1col1 := p1col1[h1 := 1];
-            } else {
                 p1col0 := p1col0[clearIdx := 0];
                 p1col1 := p1col1[clearIdx := 0];
+            } else if (activePane == 1) {
+                p1col0 := p1col0[h0 := 1];
+                p1col1 := p1col1[h1 := 1];
+                p2col0 := p2col0[clearIdx := 0];
+                p2col1 := p2col1[clearIdx := 0];
+            } else {
+                p0col0 := p0col0[clearIdx := 0];
+                p0col1 := p0col1[clearIdx := 0];
                 p2col0 := p2col0[h0 := 1];
                 p2col1 := p2col1[h1 := 1];
             }
+            lastInsertTime := lastInsertTime[key := curTs];
+            lastOpTime := curTs;
         }
-    }    
+    }
+
+    // test a single rotate with a fixed time interval between packets
+    method singleRotateTest() {
+        var prog := new Program();
+        prog.p2col0 := prog.p2col0[0 := 1]; // suppose that something is set somewhere
+        assert prog.curTs == 0;
+        // insert some key
+        prog.insert(1);
+        var n := 0;
+        while (n < 310) 
+            invariant prog.timingInvariant()
+            invariant prog.stateInvariant()
+            invariant prog.arraySizes ()
+            invariant prog.lastOpTime == prog.curTs // the loop starts just after finishing an operation
+            invariant prog.curTs == n
+            // no rotations in this loop...
+            invariant prog.tLastRotate == 0
+            invariant prog.activePane == 0            
+            invariant prog.keyExistsInActive(1)
+        {
+            // increment time
+            prog.curTs := prog.curTs + 1;
+            // do any operation
+            label PRE:
+            var _ := prog.query(1);
+            assert |old@PRE(prog.p0col0)| == |prog.p0col0|;
+            assert prog.noRemovalsInActiveOrMaintain@PRE();
+            n := n + 1;
+        }
+        assert prog.curTs == 310;
+        assert prog.keyExistsInPane(1, 0);
+        // increment time to exactly the rotate time
+        prog.curTs := prog.curTs + prog.tPktInterArrival;
+        // look for the key, which should both rotate _and_ find it.
+        var found := prog.query(1);
+        assert prog.activePane == 1;
+    }
+
+    type validTime = x : nat | 0 <= x < 10    
+
+
+    method arbitraryRotateTest() {
+        var prog := new Program();
+        prog.insert(1); // insert the test key
+        assert prog.keyExistsInPane(1, 0);
+
+        var tRemain : nat := prog.tinterval;
+        assert prog.curTs == 0;
+        assert prog.tLastRotate == 0;
+        while (tRemain > 0) 
+            invariant prog.curTs + tRemain == prog.tinterval
+            invariant prog.curTs <= prog.tinterval
+            invariant prog.timingInvariant()
+            invariant prog.stateInvariant()
+            invariant prog.arraySizes ()
+            invariant prog.lastOpTime == prog.curTs // the loop starts just after finishing an operation
+            // invariant prog.curTs < prog.tinterval;
+        {
+            var delay : uint32 := rand(1, prog.tPktInterArrival);
+            
+            delay := if (delay > tRemain)
+                then tRemain
+                else delay ;
+
+            assert prog.curTs + delay != prog.tLastRotate;
+
+            prog.curTs := prog.curTs + delay;
+            // what if this always held: curTs - lastRotate > 0 
+            // 
+            assert prog.curTs != prog.tLastRotate;
+  
+
+            var _ := prog.query(0); // noop just to maintain clearing
+            tRemain := tRemain - delay;
+        }
+        assert tRemain == 0;
+
+    }
 
 }
